Proved more examples.

ARCH2022_Examples.thy
@@ -13,6 +13,7 @@ begin
 
 subsection \<open> Basic \<close>
 
+lit_vars \<comment> \<open> disable constants \<close>
 
 subsubsection \<open> Basic assignment \<close> 
 
@@ -79,7 +80,7 @@ qed
 (* Proof using the solution *)
 (* x>=0 -> [x:=x+1;][{x'=2}]x>=1 *)
 lemma "(x \<ge> 0)\<^sub>e \<le> |x ::= x + 1] |{x` = 2}] (x \<ge> 1)"
-  apply (subst fbox_solve[where \<phi>="\<lambda>t. [x \<leadsto> 2 * \<guillemotleft>t\<guillemotright> + x]"]; simp add: wp)
+  apply (subst fbox_solve[where \<phi>="\<lambda>t. [x \<leadsto> 2 * t + x]"]; simp add: wp)
   by (local_flow 1) expr_simp
 
 (* usind differential invariants *)
@@ -123,7 +124,7 @@ begin
 
 (* x>=0 & y>=1 -> [x:=x+1;][{x:=x+1;}*@invariant(x>=1) ++ y:=x+1;][{y'=2}][x:=y;]x>=1 *)
 lemma "(x \<ge> 0 \<and> y \<ge>1)\<^sub>e \<le> |x ::= x + 1]|LOOP x ::= x + 1 INV (x \<ge> 1) \<sqinter> y ::= x + 1] |{y` = 2}] |x ::= y] (x \<ge> 1)"
-  apply (subst fbox_solve[where \<phi>="\<lambda>t. [y \<leadsto> 2 * \<guillemotleft>t\<guillemotright> + y]"]; simp)
+  apply (subst fbox_solve[where \<phi>="\<lambda>t. [y \<leadsto> 2 * t + y]"]; simp)
    apply (local_flow 1)[1]
   apply (subst change_loopI[where I="(1 \<le> x \<and> 1 \<le> y)\<^sub>e"])
   apply (subst fbox_kcomp[symmetric], rule hoare_kcomp)
@@ -165,7 +166,7 @@ lemma "(x > 0 \<and> y > 0)\<^sub>e \<le> |{x` = -x}]|LOOP x ::= x+3 INV (x > 0)
   apply (subst change_loopI[where I="(0 < $x \<and> 0 < $y)\<^sup>e"])
   apply (subst fbox_kcomp[symmetric])
   apply (rule_tac R="(0 < x \<and> 0 < y)\<^sup>e" in hoare_kcomp)
-   apply (subst fbox_solve[where \<phi>="\<lambda>t. [x \<leadsto> x * exp (- \<guillemotleft>t\<guillemotright>)]"]; clarsimp?)
+   apply (subst fbox_solve[where \<phi>="\<lambda>t. [x \<leadsto> x * exp (- t)]"]; clarsimp?)
     apply (local_flow 1)[1]
    apply expr_auto[1]
   apply (rule hoare_choice)
@@ -211,11 +212,11 @@ begin
 (* x>0 -> [{x'=5};{x'=2};{x'=x}]x>0 *)
 lemma "(x > 0)\<^sub>e \<le> |{x` = 5}; {x` = 2};{x` = x}] (x > 0)"
   apply (simp add: wp)
-   apply (subst fbox_solve[where \<phi>="\<lambda>t. [x \<leadsto> 5 * \<guillemotleft>t\<guillemotright> + x]"]; clarsimp?)
+   apply (subst fbox_solve[where \<phi>="\<lambda>t. [x \<leadsto> 5 * t + x]"]; clarsimp?)
    apply (local_flow 1)[1]
-   apply (subst fbox_solve[where \<phi>="\<lambda>t. [x \<leadsto> 2 * \<guillemotleft>t\<guillemotright> + x]"]; clarsimp?)
+   apply (subst fbox_solve[where \<phi>="\<lambda>t. [x \<leadsto> 2 * t + x]"]; clarsimp?)
    apply (local_flow 1)[1]
-  apply (subst fbox_solve[where \<phi>="\<lambda>t. [x \<leadsto> x * exp \<guillemotleft>t\<guillemotright>]"]; clarsimp?)
+  apply (subst fbox_solve[where \<phi>="\<lambda>t. [x \<leadsto> x * exp t]"]; clarsimp?)
    apply (local_flow 1)[1]
   by expr_auto
 
@@ -235,7 +236,7 @@ lemma "\<^bold>{x = 0\<^bold>} {x` = 1} \<^bold>{x \<ge> 0\<^bold>}"
 (* proof with solutions *)
 (* x=0->[{x'=1}]x>=0 *)
 lemma "\<^bold>{x = 0\<^bold>} {x` = 1} \<^bold>{x \<ge> 0\<^bold>}"
-  apply (subst fbox_solve[where \<phi>="\<lambda>t. [x \<leadsto> \<guillemotleft>t\<guillemotright> + x]"]; clarsimp?)
+  apply (subst fbox_solve[where \<phi>="\<lambda>t. [x \<leadsto> t + x]"]; clarsimp?)
   by (local_flow 1) expr_auto
 
 end
@@ -248,7 +249,7 @@ begin
 
 (* x>=0 & y>=0 -> [{x'=y}]x>=0 *)
 lemma "\<^bold>{x \<ge> 0 \<and> y \<ge> 0\<^bold>} {x` = y} \<^bold>{x \<ge> 0\<^bold>}"
-  apply (subst fbox_solve[where \<phi>="\<lambda>t. [x \<leadsto> y * \<guillemotleft>t\<guillemotright> + x]"]; clarsimp?)
+  apply (subst fbox_solve[where \<phi>="\<lambda>t. [x \<leadsto> y * t + x]"]; clarsimp?)
   by (local_flow 1) expr_auto
 
 (* x>=0 & y>=0 -> [{x'=y}]x>=0 *)
@@ -270,7 +271,7 @@ begin
 
 (* x>=0 & y>=0 & z>=0 -> [{x'=y,y'=z}]x>=0 *)
 lemma "(x \<ge> 0 \<and> y \<ge>0 \<and> z \<ge> 0)\<^sub>e \<le> |{x` = y, y` = z}] (x \<ge> 0)"
-  apply (subst fbox_solve[where \<phi>="\<lambda>t. [x \<leadsto> z * \<guillemotleft>t\<guillemotright>\<^sup>2 / 2 + y * \<guillemotleft>t\<guillemotright> + x, y \<leadsto> z * \<guillemotleft>t\<guillemotright> + y]"]; clarsimp?)
+  apply (subst fbox_solve[where \<phi>="\<lambda>t. [x \<leadsto> z * t\<^sup>2 / 2 + y * t + x, y \<leadsto> z * t + y]"]; clarsimp?)
   apply (unfold local_flow_on_def, clarsimp, unfold_locales; expr_simp)
   subgoal by (lipschitz 1) (metis norm_snd_le real_norm_def)
   by (auto intro!: poly_derivatives) expr_simp
@@ -308,7 +309,7 @@ begin
 (* proof with solutions *)
 (* x>0 -> [{x'=-x}]x>0 *)
 lemma "(x > 0)\<^sub>e \<le> |{x` = -x}] (x > 0)"
-  apply (subst fbox_solve[where \<phi>="\<lambda>t. [x \<leadsto> x * exp (- \<guillemotleft>t\<guillemotright>)]"]; clarsimp?)
+  apply (subst fbox_solve[where \<phi>="\<lambda>t. [x \<leadsto> x * exp (- t)]"]; clarsimp?)
   by (local_flow 1) expr_auto
  
 (* proof with ghosts *)
@@ -329,7 +330,7 @@ begin
 (* proof with solutions *)
 (* x>0 -> [{x'=-x+1}]x>0 *)
 lemma "(x > 0)\<^sub>e \<le> |{x` = -x + 1}] (x > 0)"
-  apply (subst fbox_solve[where \<phi>="\<lambda>t. [x \<leadsto> 1 - exp (- \<guillemotleft>t\<guillemotright>) + x * exp (- \<guillemotleft>t\<guillemotright>)]"]; clarsimp?)
+  apply (subst fbox_solve[where \<phi>="\<lambda>t. [x \<leadsto> 1 - exp (- t) + x * exp (- t)]"]; clarsimp?)
   by (local_flow 1, expr_auto) 
     (metis add_pos_nonneg diff_gt_0_iff_gt exp_eq_one_iff 
       exp_ge_zero exp_less_one_iff less_eq_real_def mult.commute mult_1 
@@ -354,7 +355,7 @@ begin
 
 (* x>0 & y>0->[{x'=-y*x}]x>0 *)
 lemma "`y > 0` \<Longrightarrow> (x > 0)\<^sub>e \<le> |{x` = - y * x}] (x > 0)"
-  apply (subst fbox_solve[where \<phi>="\<lambda>t. [x \<leadsto> x * exp (- \<guillemotleft>t\<guillemotright> * y)]"]; clarsimp?)
+  apply (subst fbox_solve[where \<phi>="\<lambda>t. [x \<leadsto> x * exp (- t * y)]"]; clarsimp?)
    apply (unfold local_flow_on_def, clarsimp, unfold_locales; expr_simp)
   subgoal for s apply (lipschitz "get\<^bsub>y\<^esub> s")
     using less_eq_real_def apply presburger
@@ -373,7 +374,7 @@ begin
 
 (* x>=0 -> [{x'=x}]x>=0 *)
 lemma "(x \<ge> 0)\<^sub>e \<le> |{x` = x}] (x \<ge> 0)"
-  apply (subst fbox_solve[where \<phi>="\<lambda>t. [x \<leadsto> x * exp \<guillemotleft>t\<guillemotright>]"]; clarsimp?)
+  apply (subst fbox_solve[where \<phi>="\<lambda>t. [x \<leadsto> x * exp t]"]; clarsimp?)
   by (local_flow 1) expr_auto 
 
 (* proof with ghosts *)
@@ -417,14 +418,14 @@ context two_vars
 begin
 
 (* x>=1 -> [{x'=x\<^sup>2+2*x^4}]x^3>=x\<^sup>2 *)
-lemma "(x \<ge> 1)\<^sub>e \<le> |{x` = x\<^sup>2 + 2 * x^4}] (x^3 \<ge> x\<^sup>2)"
+lemma "(x \<ge> 1)\<^sub>e \<le> |{x` = x\<^sup>2 + 2 * x\<^sup>4}] (x^3 \<ge> x\<^sup>2)"
   apply (rule diff_cut_on_rule[where C="(1 \<le> x)\<^sup>e"])
-   apply (diff_inv_on_ineq "(0)\<^sup>e" "(x\<^sup>2 + 2 * x^4)\<^sup>e")
-  apply (rule diff_cut_on_rule[where C="(x\<^sup>2 \<le> x^3)\<^sup>e"])
-   apply (rule fbox_inv[where I="(x\<^sup>2 \<le> x^3)\<^sup>e"])
+   apply (diff_inv_on_ineq "(0)\<^sup>e" "(x\<^sup>2 + 2 * x\<^sup>4)\<^sup>e")
+  apply (rule diff_cut_on_rule[where C="(x\<^sup>2 \<le> x\<^sup>3)\<^sup>e"])
+   apply (rule fbox_inv[where I="(x\<^sup>2 \<le> x\<^sup>3)\<^sup>e"])
      apply (expr_simp add: le_fun_def numeral_Bit1 field_simps)
   apply (simp only: expr_defs hoare_diff_inv_on fbox_diff_inv_on)
-  apply (diff_inv_on_single_ineq_intro "(2 * x * (x\<^sup>2 + 2 * x^4))\<^sup>e" "(3 * x\<^sup>2 * (x\<^sup>2 + 2 * x^4))\<^sup>e"; clarsimp)
+  apply (diff_inv_on_single_ineq_intro "(2 * x * (x\<^sup>2 + 2 * x\<^sup>4))\<^sup>e" "(3 * x\<^sup>2 * (x\<^sup>2 + 2 * x\<^sup>4))\<^sup>e"; clarsimp)
      apply(auto intro!: poly_derivatives simp: field_simps semiring_normalization_rules(27,28))[1]
   subgoal for X \<tau>
     apply (move_left "2::real", move_left "3::real", move_left "4::real", move_left "6::real")
@@ -488,9 +489,9 @@ begin
 (* d1\<^sup>2+d2\<^sup>2=w\<^sup>2*p\<^sup>2 & d1=-w*x2 & d2=w*x1 -> 
   [{x1'=d1, x2'=d2, d1'=-w*d2, d2'=w*d1}]
   (d1\<^sup>2+d2\<^sup>2=w\<^sup>2*p\<^sup>2 & d1=-w*x2 & d2=w*x1)*)
-lemma "(d1\<^sup>2 + d2\<^sup>2 = \<guillemotleft>w\<guillemotright>\<^sup>2 * \<guillemotleft>p\<guillemotright>\<^sup>2 \<and> d1 = - \<guillemotleft>w\<guillemotright> * x2 \<and> d2 = \<guillemotleft>w\<guillemotright> * x1)\<^sub>e \<le>
-  |{x1` = d1, x2` = d2, d1` = - \<guillemotleft>w\<guillemotright> * d2, d2` = \<guillemotleft>w\<guillemotright> * d1}] 
-  (d1\<^sup>2 + d2\<^sup>2 = \<guillemotleft>w\<guillemotright>\<^sup>2 * \<guillemotleft>p\<guillemotright>\<^sup>2 \<and> d1 = - \<guillemotleft>w\<guillemotright> * x2 \<and> d2 = \<guillemotleft>w\<guillemotright> * x1)"
+lemma "(d1\<^sup>2 + d2\<^sup>2 = w\<^sup>2 * p\<^sup>2 \<and> d1 = - w * x2 \<and> d2 = w * x1)\<^sub>e \<le>
+  |{x1` = d1, x2` = d2, d1` = - w * d2, d2` = w * d1}] 
+  (d1\<^sup>2 + d2\<^sup>2 = w\<^sup>2 * p\<^sup>2 \<and> d1 = - w * x2 \<and> d2 = w * x1)"
   by (rule fbox_invs; (rule fbox_invs)?) diff_inv_on_eq+
 
 end
@@ -650,14 +651,14 @@ context two_vars
 begin
 
 (* x^3>5 & y>2 -> [{x'=x^3+x^4, y'=5*y+y^2}](x^3>5 & y>2) *)
-lemma "(x^3 > 5 \<and> y > 2)\<^sub>e \<le> |{x` = x^3 + x^4, y` = 5*y + y\<^sup>2}] (x^3 > 5 \<and> y > 2)"
+lemma "(x\<^sup>3 > 5 \<and> y > 2)\<^sub>e \<le> |{x` = x\<^sup>3 + x\<^sup>4, y` = 5*y + y\<^sup>2}] (x\<^sup>3 > 5 \<and> y > 2)"
   apply (rule fbox_invs; (rule fbox_invs)?)
   apply (expr_simp)
   apply (clarsimp simp only: fbox_diff_inv_on diff_inv_on_eq ivp_sols_def)
    apply (expr_simp add: Collect_ge_ivl)
   subgoal for s X t
-    apply(rule current_vderiv_ge_always_ge[of 5 "\<lambda>t. (fst (X t)) ^ 3" 0 
-        "\<lambda>t. 3 * (fst (X t)) ^ 2 * (fst (X t) ^ 3 + fst (X t) ^ 4)", where g="\<lambda>t. 3 * t^2 + 3 * (root 3 t)^5", rule_format])
+    apply(rule current_vderiv_ge_always_ge[of 5 "\<lambda>t. (fst (X t))\<^sup>3" 0 
+        "\<lambda>t. 3 * (fst (X t))\<^sup>2 * ((fst (X t))\<^sup>3 + (fst (X t))\<^sup>4)", where g="\<lambda>t. 3 * t\<^sup>2 + 3 * (root 3 t)\<^sup>5", rule_format])
     by (auto intro!: poly_derivatives simp: odd_real_root_power_cancel split: if_splits) 
       (distribute, mon_pow_simp, force)
   apply (clarsimp simp only: fbox_diff_inv_on diff_inv_on_eq ivp_sols_def)
@@ -690,9 +691,9 @@ end
 
 subsubsection \<open> Dynamics: Conserved quantity \<close>
 
-lemma dyn_cons_qty_arith: "(36::real) * (x1\<^sup>2 * (x1 * x2 ^ 3)) - 
-  (- (24 * (x1\<^sup>2 * x2) * x1 ^ 3 * (x2)\<^sup>2) - 12 * (x1\<^sup>2 * x2) * x1 * x2 ^ 4) - 
-  36 * (x1\<^sup>2 * (x2 * x1)) * (x2)\<^sup>2 - 12 * (x1\<^sup>2 * (x1 * x2 ^ 5)) = 24 * (x1 ^ 5 * x2 ^ 3)" 
+lemma "(36::real) * (x1\<^sup>2 * (x1 * x2\<^sup>3)) - 
+  (- (24 * (x1\<^sup>2 * x2) * x1 ^ 3 * (x2)\<^sup>2) - 12 * (x1\<^sup>2 * x2) * x1 * x2\<^sup>4) - 
+  36 * (x1\<^sup>2 * (x2 * x1)) * (x2)\<^sup>2 - 12 * (x1\<^sup>2 * (x1 * x2\<^sup>5)) = 24 * (x1\<^sup>5 * x2\<^sup>3)" 
   by (mon_simp_vars x1 x2)
 
 dataspace conserved_quantity =
@@ -705,9 +706,9 @@ begin
 (* x1^4*x2^2+x1^2*x2^4-3*x1^2*x2^2+1 <= c ->
     [{x1'=2*x1^4*x2+4*x1^2*x2^3-6*x1^2*x2, x2'=-4*x1^3*x2^2-2*x1*x2^4+6*x1*x2^2}] 
    x1^4*x2^2+x1^2*x2^4-3*x1^2*x2^2+1 <= c *)
-lemma "(x1^4*x2\<^sup>2 + x1\<^sup>2*x2^4 - 3*x1\<^sup>2*x2\<^sup>2 + 1 \<le> \<guillemotleft>c\<guillemotright>)\<^sub>e \<le>
-  |{x1` = 2*x1^4*x2 + 4*x1^2*x2^3 - 6*x1\<^sup>2*x2, x2` = -4*x1^3*x2\<^sup>2 - 2*x1*x2^4 + 6*x1*x2\<^sup>2}]
-  (x1^4*x2\<^sup>2 + x1\<^sup>2*x2^4 - 3*x1\<^sup>2*x2\<^sup>2 + 1 \<le> \<guillemotleft>c\<guillemotright>)"
+lemma "(x1\<^sup>4*x2\<^sup>2 + x1\<^sup>2*x2\<^sup>4 - 3*x1\<^sup>2*x2\<^sup>2 + 1 \<le> c)\<^sub>e \<le>
+  |{x1` = 2*x1\<^sup>4*x2 + 4*x1\<^sup>2*x2\<^sup>3 - 6*x1\<^sup>2*x2, x2` = -4*x1\<^sup>3*x2\<^sup>2 - 2*x1*x2\<^sup>4 + 6*x1*x2\<^sup>2}]
+  (x1\<^sup>4*x2\<^sup>2 + x1\<^sup>2*x2\<^sup>4 - 3*x1\<^sup>2*x2\<^sup>2 + 1 \<le> c)"
   apply (simp only: expr_defs hoare_diff_inv_on fbox_diff_inv_on)
   apply (diff_inv_on_single_ineq_intro "(0)\<^sup>e" "(0)\<^sup>e"; expr_simp)
   apply (intro poly_derivatives; (assumption)?, (rule poly_derivatives)?)
@@ -772,7 +773,7 @@ context darboux
 begin
 
 (* x+z=0 -> [{x'=(A*x^2+B()*x), z' = A*z*x+B()*z}] 0=-x-z *)
-lemma "(x + z = 0)\<^sub>e \<le> |{x` = \<guillemotleft>A\<guillemotright>*x\<^sup>2 + \<guillemotleft>B\<guillemotright>*x, z` = \<guillemotleft>A\<guillemotright>*z*x+\<guillemotleft>B\<guillemotright>*z | G on UNIV UNIV @ 0}] (0= -x - z)"
+lemma "(x + z = 0)\<^sub>e \<le> |{x` = A*x\<^sup>2 + \<guillemotleft>B\<guillemotright>*x, z` = A*z*x+B*z | G on UNIV UNIV @ 0}] (0= -x - z)"
   apply (subgoal_tac "(0= -x - z)\<^sup>e = (x + z = 0)\<^sup>e"; force?)
   apply (erule ssubst)
   apply (simp only: expr_defs hoare_diff_inv_on fbox_diff_inv_on fbox_diff_inv_on')
@@ -784,20 +785,19 @@ lemma "(x + z = 0)\<^sub>e \<le> |{x` = \<guillemotleft>A\<guillemotright>*x\<^s
       apply (distribute, mon_pow_simp)
      prefer 2 apply (force intro!: poly_derivatives)
     apply (unfold_locales; clarsimp?)
-     apply (force intro!: continuous_intros vderiv_on_continuous_on poly_derivatives)
+     apply (force intro!: vderiv_on_continuous_on poly_derivatives)
     apply distribute
     apply (rule_tac f'="\<lambda>(t, r). Blinfun (\<lambda>r. r * (A * fst (X t)) + r * B) " in c1_implies_local_lipschitz; clarsimp?)
     apply (rule has_derivative_Blinfun)
-     apply (auto intro!: derivative_eq_intros continuous_intros vderiv_on_continuous_on split: prod.splits)[1]
+     apply (auto intro!: derivative_eq_intros vderiv_on_continuous_on split: prod.splits)[1]
     apply (rule continuous_on_blinfun_componentwise)
     apply (simp add: prod.case_eq_if)
     apply (subst bounded_linear_Blinfun_apply)
     subgoal for i w
       apply (rule_tac f="(\<lambda>r. r * (A * fst (X (fst w))) + r * B)" in has_derivative_bounded_linear)
       by (auto intro!: derivative_eq_intros)
-    apply (auto intro!: continuous_intros)[1]
-    apply (rule continuous_on_compose[of UNIV fst X, unfolded comp_def])
-    by (auto intro!: continuous_intros vderiv_on_continuous_on)
+    by (auto intro!: continuous_intros vderiv_on_continuous_on
+        continuous_on_compose[of UNIV fst X, unfolded comp_def] )
   done
 
 end
@@ -809,30 +809,29 @@ context darboux
 begin
 
 (* x+z=0 -> [{x'=(A*y+B()*x)/z^2, z' = (A*x+B())/z & y = x^2 & z^2 > 0}] x+z=0 *)
-lemma "(x + z = 0)\<^sub>e \<le> |{x` = (\<guillemotleft>A\<guillemotright>*y + \<guillemotleft>B\<guillemotright>*x)/z\<^sup>2, z` = (\<guillemotleft>A\<guillemotright>*x+\<guillemotleft>B\<guillemotright>)/z | (y = x\<^sup>2 \<and> z\<^sup>2 > 0) on UNIV UNIV @ 0}] (x + z = 0)"
+lemma "(x + z = 0)\<^sub>e \<le> |{x` = (A*y + B*x)/z\<^sup>2, z` = (A*x+B)/z | (y = x\<^sup>2 \<and> z\<^sup>2 > 0)}] (x + z = 0)"
   apply (simp only: expr_defs hoare_diff_inv_on fbox_diff_inv_on fbox_diff_inv_on')
   apply (expr_simp add: diff_inv_on_eq ivp_sols_def, clarsimp)
   subgoal for s X t
-    apply (rule picard_lindeloef.ivp_unique_solution[of "(\<lambda>t r. r * (A * (fst (X t)) + B))" UNIV UNIV 0 "get\<^bsub>x\<^esub> s + get\<^bsub>z\<^esub> s" "\<lambda>s. UNIV" t 
-          _ "\<lambda>t. 0"]; (clarsimp simp: ivp_sols_def)?)
+    apply (rule picard_lindeloef.ivp_unique_solution[of "(\<lambda>t r. r * (A * (fst (X t)) + B)/(snd (X t))\<^sup>2)" 
+          "(Collect ((\<le>) 0))" UNIV 0 "get\<^bsub>x\<^esub> s + get\<^bsub>z\<^esub> s" "\<lambda>s. {0--t}" t 
+          _ "\<lambda>t. 0"]; (clarsimp simp: ivp_sols_def closed_segment_eq_real_ivl)?)
+      prefer 3 subgoal
+      apply (frule has_vderiv_on_subset[where T="{0..t}"]; clarsimp?)
+      by (force intro!: poly_derivatives)
+    prefer 2 subgoal
+      apply (frule has_vderiv_on_subset[where T="{0..t}"]; clarsimp?)
+      by (auto simp: field_simps intro!: poly_derivatives)
+    apply (unfold_locales; clarsimp?) \<comment> \<open> set is not open \<close>
     oops
-(* see if it can be solved as above, otherwise check if diff-ghosts works, otherwise 
-  requires picard-lindeloef for closed intervals *)
+
+value "2 \<noteq> 2"
+(* check if diff-ghosts works (darboux tactic), otherwise requires picard-lindeloef for closed intervals *)
 
 end
 
+
 subsubsection \<open> Dynamics: Darboux inequality \<close> (*N 31 *)
-
-abbreviation darboux_ineq_f :: "real^2 \<Rightarrow> real^2" ("f")
-  where "f s \<equiv> (\<chi> i. if i=1 then (s$1)^2 else (s$2)*(s$1)+(s$1)^2)"
-
-abbreviation darboux_ineq_flow2 :: "real \<Rightarrow> real^2 \<Rightarrow> real^2" ("\<phi>")
-  where "\<phi> t s \<equiv> (\<chi> i. if i=1 then (s$1/(1 - t * s$1)) else
-      (s$2 - s$1 * ln(1 - t * s$1))/(1 - t * s$1))"
-
-lemma darboux_flow_ivp: "(\<lambda>t. \<phi> t s) \<in> Sols (\<lambda>s. {t. 0 \<le> t \<and> t * s $ 1 < 1}) UNIV (\<lambda>t. f) 0 s"
-  by (rule ivp_solsI) (auto intro!: poly_derivatives 
-      simp: forall_2 add_divide_distrib power_divide vec_eq_iff power2_eq_square)
 
 lemma darboux_ineq_arith:
   assumes "0 \<le> s\<^sub>1 + s\<^sub>2" and "0 \<le> (t::real)" and "t * s\<^sub>1 < 1"
@@ -862,28 +861,67 @@ proof-
     by (metis (full_types) add_diff_eq add_divide_distrib order_trans)
 qed
 
-context three_vars
+(* directly annotating the dynamics *)
+locale darboux_ineq =
+  fixes x::"real \<Longrightarrow> real^2"
+    and y::real
+    and z::"real \<Longrightarrow> real^2"
+  assumes var_defs:
+    "x \<equiv> vec_lens 1"
+    "z \<equiv> vec_lens 2"
 begin
 
+lemma indeps: "x \<bowtie> z"
+  unfolding var_defs
+  by expr_auto+
+
+lemma induct_2: "P 1 \<Longrightarrow> P 2 \<Longrightarrow> P (i::2)"
+  using exhaust_2[of i]
+  by auto
+
 (* x+z>=0 -> [{x'=x^2, z' = z*x+y & y = x^2}] x+z>=0 *)
-lemma "(x + z \<ge> 0)\<^sub>e \<le> |{x` = x\<^sup>2, z` = z*x + y | y = x\<^sup>2}] (x + z \<ge> 0)"
-  apply (subst fbox_solve[where \<phi>=""])
-  oops
+abbreviation (input) darboux_ineq_f2 :: "real ^ 2 \<Rightarrow> real ^ 2" ("f")
+  where "f \<equiv> [x \<leadsto> x\<^sup>2, z \<leadsto> z*x + x\<^sup>2]"
+
+abbreviation darboux_ineq_flow2 :: "real \<Rightarrow> real ^ 2 \<Rightarrow> real ^ 2" ("\<phi>")
+  where "\<phi> t \<equiv> [x \<leadsto> x / (1 - t * x), z \<leadsto> (z - x * ln(1 - t * x))/(1 - t * x)]"
+
+lemma darboux_flow_ivp: "(\<lambda>t. \<phi> t s) \<in> Sols ({t. 0 \<le> t \<and> t * x < 1})\<^sub>e UNIV (\<lambda>t. f) 0 s"
+  apply (rule ivp_solsI; expr_auto add: var_defs)
+  subgoal for i
+  using var_defs exhaust_2[of i]
+  by (cases "i=2"; cases "i=1")
+    (auto simp: expr_simps lens_defs vec_upd_def fun_eq_iff
+      add_divide_distrib power2_eq_square
+      intro!: poly_derivatives split: if_splits)
+  done
+
+(* x+z>=0 -> [{x'=x^2, z' = z*x+y & y = x^2}] x+z>=0 *)
+lemma "(x + z \<ge> 0)\<^sub>e \<le> |EVOL \<phi> (y = x\<^sup>2)\<^sub>e ({t. 0 \<le> t \<and> t * x < 1})\<^sub>e] (x + z \<ge> 0)"
+  apply (subst fbox_g_evol)
+  using var_defs darboux_ineq_arith
+  by (clarsimp simp: expr_simps expr_defs)
+
+no_notation darboux_ineq_f2 ("f") 
+  and darboux_ineq_flow2 ("\<phi>")
 
 end
 
+context three_vars
+begin
+
+(* attempt by providing solutions *)
 (* x+z>=0 -> [{x'=x^2, z' = z*x+y & y = x^2}] x+z>=0 *)
-(* x' + z' \<ge> 0 \<longleftrightarrow> x^2 + z*x + x^2 \<ge> 0*)
-lemma "(\<lambda>s::real^2. s$1 + s$2 \<ge> 0) \<le> 
-  |EVOL \<phi> (\<lambda>s. y = (s$1)^2) (\<lambda>s. {t. 0 \<le> t \<and> t * s $ 1 < 1})]
-  (\<lambda>s. s$1 + s$2 \<ge> 0)"
-  apply(subst fbox_g_evol, simp_all add: le_fun_def)
-  using darboux_ineq_arith by smt
+lemma "(x + z \<ge> 0)\<^sub>e \<le> |{x` = x\<^sup>2, z` = z*x + y | y = x\<^sup>2}] (x + z \<ge> 0)"
+  apply (subst fbox_g_ode_frame_flow[where 
+        \<phi>="\<lambda>t. [x \<leadsto> x / (1 - t * x), z \<leadsto> (z - x * ln(1 - t * x))/(1 - t * x)]"])
+  subgoal 
+    apply (unfold local_flow_on_def, clarsimp)
+    apply (unfold_locales; expr_simp)
+    prefer 5 apply (auto simp: intro!: poly_derivatives)[1]
+  oops (* local_flow's interval parameter should be a function *)
 
-no_notation darboux_ineq_flow2 ("\<phi>")
-        and darboux_ineq_f ("f")
-
-(* interval of existence or invariant rule for \<le> *)
+end
 
 
 subsubsection \<open> Dynamics: Bifurcation \<close>
@@ -912,31 +950,39 @@ proof(unfold_locales; clarsimp simp: dist_norm local_lipschitz_def lipschitz_on_
     by (rule_tac x=1 in exI, clarsimp, rule_tac x="2 * (1 + \<bar>x\<bar>)" in exI, auto)
 qed
 
+context two_vars
+begin
+
 (* r <= 0 -> \exists f (x=f -> [{x'=r+x^2}]x=f) *)
-lemma "r \<le> 0 \<Longrightarrow> \<exists>c. (\<lambda>s::real^1. s$1 = c) \<le> 
-  |x\<acute>= (\<lambda>t s. (\<chi> i. r + (s$1)^2)) & G on (\<lambda>s. UNIV) UNIV @ 0] 
-  (\<lambda>s. s$1 = c)"
-proof(rule_tac x="sqrt \<bar>r\<bar>" in exI, clarsimp simp: diff_inv_eq ivp_sols_def)
-  fix X::"real\<Rightarrow>real^1" and t::real
-  assume init: "X 0 $ 1 = sqrt (- r)" and "r \<le> 0"
-     and D1: "D (\<lambda>x. X x $ 1) = (\<lambda>x. r + (X x $ 1)\<^sup>2) on UNIV"
-  hence "D (\<lambda>x. X x $ 1) = (\<lambda>x. r + (X x $ 1)\<^sup>2) on {0--t}"
-    using has_vderiv_on_subset by blast
-  moreover have "continuous_on UNIV (\<lambda>t. X t $ 1)"
+lemma 
+  fixes r::real
+  shows "`\<guillemotleft>r\<guillemotright> \<le> 0` \<longrightarrow> (\<exists>f. (x=f)\<^sub>e \<le> |{x` = \<guillemotleft>r\<guillemotright> + x^2| True on UNIV UNIV @ 0}] (x=f))"
+proof(clarsimp, rule_tac x="sqrt \<bar>r\<bar>" in exI, clarsimp simp: hoare_diff_inv_on diff_inv_on_eq ivp_sols_def)
+  fix X::"real\<Rightarrow>real" and t::real and s::'st
+  assume init: "X 0 = sqrt \<bar>r\<bar>" and "`r \<le> 0`"
+     and D1: "D X = (\<lambda>t. get\<^bsub>x\<^esub> ([x \<leadsto> \<guillemotleft>r\<guillemotright> + ($x)\<^sup>2] (put\<^bsub>x\<^esub> s (X t)))) on UNIV"
+  have "D X = (\<lambda>t. get\<^bsub>x\<^esub> ([x \<leadsto> \<guillemotleft>r\<guillemotright> + ($x)\<^sup>2] (put\<^bsub>x\<^esub> s (X t)))) on {0--t}"
+    apply(rule has_vderiv_on_subset[OF D1])
+    by (auto simp: closed_segment_eq_real_ivl)
+  moreover have "continuous_on UNIV X"
     apply(rule vderiv_on_continuous_on)
     using D1 by assumption
   moreover have key: "D (\<lambda>t. sqrt (- r)) = (\<lambda>t. r + (sqrt (- r))\<^sup>2) on {0--t}"
     apply(subgoal_tac "(\<lambda>t. r + (sqrt (- r))\<^sup>2) = (\<lambda>t. 0)")
      apply(erule ssubst, rule poly_derivatives)
-    using \<open>r \<le> 0\<close> by auto
+    using \<open>`r \<le> 0`\<close> by expr_auto
   moreover note picard_lindeloef.ivp_unique_solution[OF 
       picard_lindeloef_dyn_bif[OF calculation(2) UNIV_I is_interval_univ open_UNIV] 
       UNIV_I is_interval_closed_segment_1 subset_UNIV _ 
-      ivp_solsI[of "\<lambda>x. X x $ 1" _ "\<lambda>s. {0--t}" "sqrt (- r)" 0]
+      ivp_solsI[of "X" _ "\<lambda>s. {0--t}" "sqrt (- r)" 0]
       ivp_solsI[of "\<lambda>t. sqrt (- r)" _], of t r]
-  ultimately show "X t $ 1 = sqrt (- r)"
-    using \<open>r \<le> 0\<close> init by auto
+  ultimately show "X t = sqrt \<bar>r\<bar>"
+    using \<open>`r \<le> 0`\<close> init
+    by expr_auto
 qed
+
+end
+
 
 subsubsection \<open> Dynamics: Parametric switching between two different damped oscillators \<close> (*N 33 *)
 
@@ -954,6 +1000,7 @@ subsubsection \<open> Dynamics: Parametric switching between two different dampe
   ] w^2*x^2+y^2 <= c *)
 
 (* verified with the help of a CAS *)
+value "2 \<noteq> 2"
 
 
 subsubsection \<open> Dynamics: Nonlinear 1 \<close>
@@ -965,8 +1012,8 @@ dataspace dyn_nonlinear =
 context dyn_nonlinear
 begin
 (* x^3 >= -1 -> [{x'=(x-3)^4+a & a>=0}] x^3>=-1 *)
-lemma "(x1^3 \<ge> -1)\<^sub>e \<le> |{x1` = (x1-3)^4 + \<guillemotleft>a\<guillemotright> | (\<guillemotleft>a\<guillemotright>\<ge>0)}] (x1^3 \<ge> -1)"
-  by (diff_inv_on_ineq "(0)\<^sup>e" "(3*x1\<^sup>2*((x1-3)^4 + \<guillemotleft>a\<guillemotright>))\<^sup>e")
+lemma "(x1\<^sup>3 \<ge> -1)\<^sub>e \<le> |{x1` = (x1-3)\<^sup>4 + a | (a\<ge>0)}] (x1\<^sup>3 \<ge> -1)"
+  by (diff_inv_on_ineq "(0)\<^sup>e" "(3*x1\<^sup>2*((x1-3)\<^sup>4 + a))\<^sup>e")
 
 end
 
@@ -977,11 +1024,10 @@ context dyn_nonlinear
 begin
 
 (* x1+x2^2/2=a -> [{x1'=x1*x2,x2'=-x1}]x1+x2^2/2=a *)
-lemma "(x1 + x2\<^sup>2/2 = \<guillemotleft>a\<guillemotright>)\<^sub>e \<le> |{x1` = x1 * x2, x2` = -x1}] (x1 + x2\<^sup>2/2 = \<guillemotleft>a\<guillemotright>)"
+lemma "(x1 + x2\<^sup>2/2 = a)\<^sub>e \<le> |{x1` = x1 * x2, x2` = -x1}] (x1 + x2\<^sup>2/2 = a)"
   by (diff_inv_on_eq)
 
 end
-
 
 
 subsubsection \<open> Dynamics: Nonlinear 4 \<close>
@@ -990,7 +1036,7 @@ context dyn_nonlinear
 begin
 
 (* x1^2/2-x2^2/2>=a -> [{x1'=x2+x1*x2^2, x2'=-x1+x1^2*x2 & x1>=0 & x2>=0}]x1^2/2-x2^2/2>=a *)
-lemma "(x1\<^sup>2/2 - x2\<^sup>2/2 \<ge> \<guillemotleft>a\<guillemotright>)\<^sub>e \<le> |{x1` = x2 + x1*x2\<^sup>2, x2` = -x1 + x1\<^sup>2 * x2| (x1 \<ge> 0 \<and> x2 \<ge> 0)}] (x1\<^sup>2/2 - x2\<^sup>2/2 \<ge> \<guillemotleft>a\<guillemotright>)"
+lemma "(x1\<^sup>2/2 - x2\<^sup>2/2 \<ge> a)\<^sub>e \<le> |{x1` = x2 + x1*x2\<^sup>2, x2` = -x1 + x1\<^sup>2 * x2| (x1 \<ge> 0 \<and> x2 \<ge> 0)}] (x1\<^sup>2/2 - x2\<^sup>2/2 \<ge> a)"
   apply (simp only: expr_defs hoare_diff_inv_on fbox_diff_inv_on)
   apply (diff_inv_on_single_ineq_intro "(0)\<^sup>e" "(x1 * (x2 + x1*x2\<^sup>2) - x2 * (-x1 + x1\<^sup>2 * x2))\<^sup>e"; expr_simp)
   by (auto simp: field_simps fun_eq_iff intro!: poly_derivatives split: if_splits)
@@ -1004,7 +1050,7 @@ context dyn_nonlinear
 begin
 
 (* -x1*x2>=a -> [{x1'=x1-x2+x1*x2, x2'=-x2-x2^2}]-x1*x2>=a *)
-lemma "(-x1*x2 \<ge> \<guillemotleft>a\<guillemotright>)\<^sub>e \<le> |{x1` = x1 - x2 + x1*x2, x2` = -x2 - x2\<^sup>2}] (-x1*x2 \<ge> \<guillemotleft>a\<guillemotright>)"
+lemma "(-x1*x2 \<ge> a)\<^sub>e \<le> |{x1` = x1 - x2 + x1*x2, x2` = -x2 - x2\<^sup>2}] (-x1*x2 \<ge> a)"
   apply (simp only: expr_defs hoare_diff_inv_on fbox_diff_inv_on)
   by (diff_inv_on_single_ineq_intro "(0)\<^sup>e" "((- x1 + x2 - x1*x2)*x2 - x1 * (-x2 - x2\<^sup>2))\<^sup>e"; expr_simp)
     (auto simp: field_simps fun_eq_iff intro!: poly_derivatives split: if_splits)
@@ -1014,42 +1060,94 @@ end
 
 subsubsection \<open> Dynamics: Riccati \<close>
 
+context two_vars
+begin
+
 (* 2*x^3 >= 1/4 -> [{x'=x^2+x^4}] 2*x^3>=1/4 *)
-lemma "(\<lambda>s::real^1. 2 * s$1^3 \<ge> 1/4) \<le> 
-  |x\<acute>= (\<lambda>s. \<chi> i. s$1^2 + s$1^4) & G]
-  (\<lambda>s. 2 * s$1^3 \<ge> 1/4)"
-  apply(simp, rule_tac \<nu>'="\<lambda>s. 0" and \<mu>'="\<lambda>s. 24 * (s$1^2) * (s$1^2 + s$1^4)" in diff_inv_rules(2); clarsimp)
-  by (auto intro!: poly_derivatives simp: field_simps)
+lemma "(2*x\<^sup>3 \<ge> 1/4)\<^sub>e \<le> |{x` = x\<^sup>2 + x^4}] (2*x\<^sup>3 \<ge> 1/4)"
+  by (diff_inv_on_ineq "(0)\<^sup>e" "(6*x\<^sup>2*(x\<^sup>2 + x^4))\<^sup>e")
+
+end
 
 
 subsubsection \<open> Dynamics: Nonlinear differential cut \<close>
 
+context two_vars
+begin
+
+(* apply (subst fbox_solve[where \<phi>="\<lambda>t. [x \<leadsto> x * exp t]"]; clarsimp?) *)
+term "\<lambda>t. [y \<leadsto> y/(1 - y * t)]"
+term "(x\<^sup>4 - 12 * x\<^sup>3 + 54 * x\<^sup>2 - 108 * x + 81)\<^sub>e"
+
 (* x^3 >= -1 & y^5 >= 0 -> [{x'=(x-3)^4+y^5, y'=y^2}] (x^3 >= -1 & y^5 >= 0) *)
-lemma "(\<lambda>s::real^2. s$1^3 \<ge> - 1 \<and> s$2^5 \<ge> 0) \<le> 
-  |x\<acute>= (\<lambda>s. \<chi> i. if i=1 then (s$1 - 3)^4 else s$2^2) & G]
-  (\<lambda>s. s$1^3 \<ge> - 1 \<and> s$2^5 \<ge> 0)"
-  apply(simp, rule diff_inv_rules)
-   apply(rule_tac \<nu>'="\<lambda>s. 0" and \<mu>'="\<lambda>s. 3 * s$1^2 * (s$1 - 3)^4" in diff_inv_rules(2))
-   apply(simp_all add: forall_2, force intro!: poly_derivatives)
-   apply(rule_tac \<nu>'="\<lambda>s. 0" and \<mu>'="\<lambda>s. s$2^2" in diff_inv_rules(2))
-  by (auto intro!: diff_inv_rules poly_derivatives simp: forall_2)
+lemma "(x\<^sup>3 \<ge> -1 \<and> y\<^sup>5 \<ge> 0)\<^sub>e \<le> |{x` = (x-3)\<^sup>4+y\<^sup>5, y` = y\<^sup>2}] (x\<^sup>3 \<ge> -1 \<and> y\<^sup>5 \<ge> 0)"
+  apply (diff_cut_ineq "(0 \<le> y\<^sup>5)\<^sup>e" "(0)\<^sup>e" "(5*y\<^sup>4*y\<^sup>2)\<^sup>e")
+  apply (diff_cut_ineq "(-1 \<le> x\<^sup>3)\<^sup>e" "(0)\<^sup>e" "(3*x\<^sup>2*((x-3)\<^sup>4+y\<^sup>5))\<^sup>e")
+  by (rule diff_weak_on_rule, expr_auto)
+
+end
 
 
 subsubsection \<open> STTT Tutorial: Example 1 \<close>
 
-(* v >= 0 & A > 0 -> [ { x' = v, v' = A } ] v >= 0 *)
-lemma "A > 0 \<Longrightarrow> (\<lambda>s::real^2. s$2 \<ge> 0) \<le> 
-  |x\<acute>= (\<lambda>s. \<chi> i. if i=1 then s$2 else A) & G]
-  (\<lambda>s. s$2 \<ge> 0)"
-  apply(subst local_flow.fbox_g_ode_subset[where T="UNIV" 
-        and \<phi>="\<lambda>t s. \<chi> i::2. if i=1 then A * t^2/2 + s$2 * t + s$1 else A * t + s$2"])
-      apply(unfold_locales, simp_all add: local_lipschitz_def forall_2 lipschitz_on_def)
-    apply(clarsimp, rule_tac x=1 in exI)+
-  apply(clarsimp simp: dist_norm norm_vec_def L2_set_def)
-  unfolding UNIV_2 using exhaust_2 by (auto intro!: poly_derivatives simp: vec_eq_iff)
+dataspace STTT =
+  constants A::real B::real S::real V::real \<epsilon>::real
+  variables x::real v::real a::real c::real
+
+context STTT
+begin
+
+lemma "(v \<ge> 0 \<and> A > 0)\<^sub>e \<le> |{x` = v, v` = A}] (v \<ge> 0)"
+  apply (rule diff_cut_on_rule[where C="(0 \<le> A)\<^sup>e"])
+   apply (rule fbox_inv[where I="(0 \<le> A)\<^sup>e"])
+     apply (expr_simp add: le_fun_def)
+    apply (diff_inv_on_ineq "(0)\<^sup>e" "(0)\<^sup>e")
+   apply vderiv
+  apply (diff_cut_ineq "(0 \<le> v)\<^sup>e" "(0)\<^sup>e" "(A)\<^sup>e")
+  by (rule diff_weak_on_rule, expr_auto)
+
+end
 
 
 subsubsection \<open> STTT Tutorial: Example 2 \<close>
+
+context STTT
+begin
+
+lemma "local_flow_on [x \<leadsto> v, v \<leadsto> a, a \<leadsto> 0] (x +\<^sub>L v +\<^sub>L a) UNIV UNIV 
+  (\<lambda>t. [x \<leadsto> a * t\<^sup>2 / 2 + v * t + x, v \<leadsto> a * t + v, a \<leadsto> a])"
+  apply (clarsimp simp add: local_flow_on_def)
+  apply (unfold_locales; clarsimp?)
+  subgoal for s
+    apply (rule c1_implies_local_lipschitz[of UNIV UNIV _
+      "(\<lambda>(t,c). Blinfun (\<lambda>c. get\<^bsub>x +\<^sub>L v +\<^sub>L a\<^esub> ([x \<leadsto> $v, v \<leadsto> $a, a \<leadsto> 0] (put\<^bsub>x +\<^sub>L v +\<^sub>L a\<^esub> s c))))"])
+    by expr_simp (auto intro!: has_derivative_Blinfun derivative_eq_intros vderiv_on_continuous_on
+        fun_eq_iff continuous_intros split: prod.splits)
+  apply expr_simp
+  by (auto intro!: poly_derivatives) expr_simp
+
+lemma "local_flow_on [x \<leadsto> v, v \<leadsto> a, a \<leadsto> 0] (x +\<^sub>L v +\<^sub>L a) UNIV UNIV 
+  (\<lambda>t. [x \<leadsto> a * t\<^sup>2 / 2 + v * t + x, v \<leadsto> a * t + v, a \<leadsto> a])"
+  apply (clarsimp simp add: local_flow_on_def)
+  apply (unfold_locales; expr_simp)
+   apply (rule c1_implies_local_lipschitz[of UNIV UNIV _ 
+        "(\<lambda>(t::real,c). Blinfun (\<lambda>c. ((fst (snd c)), (snd (snd c)), 0)))"]; expr_simp)
+  by (auto intro!: has_derivative_Blinfun derivative_eq_intros poly_derivatives)
+
+lemma "local_flow_on [v \<leadsto> $a, x \<leadsto> $v] (x +\<^sub>L v) UNIV UNIV 
+  (\<lambda>t. [x \<leadsto> $a * t\<^sup>2 / 2 + $v * t + $x, v \<leadsto> $a * t + $v])"
+  apply (clarsimp simp add: local_flow_on_def)
+  apply (unfold_locales; expr_simp)
+   apply (rule c1_implies_local_lipschitz[of UNIV UNIV _ "(\<lambda>(t::real,c). Blinfun (\<lambda>c. ((snd c), 0)))"])
+  by (auto intro!: has_derivative_Blinfun derivative_eq_intros poly_derivatives)
+
+lemma local_flow_STTT: "local_flow_on [v \<leadsto> $a, x \<leadsto> $v] (x +\<^sub>L v) UNIV UNIV 
+  (\<lambda>t. [x \<leadsto> $a * t\<^sup>2 / 2 + $v * t + $x, v \<leadsto> $a * t + $v])"
+  apply (clarsimp simp add: local_flow_on_def)
+  apply (unfold_locales; expr_simp)
+  apply (clarsimp simp: local_lipschitz_def lipschitz_on_def, rule_tac x=1 in exI)+
+    apply (expr_simp, clarsimp simp: dist_norm split: prod.splits)
+  by (metis norm_snd_le real_norm_def) (expr_simp, vderiv)
 
 (* v >= 0 & A > 0 & B > 0 -> 
   [
@@ -1057,40 +1155,18 @@ subsubsection \<open> STTT Tutorial: Example 2 \<close>
       { x' = v, v' = a & v >= 0 }
     }*@invariant(v >= 0)
   ] v >= 0 *)
+lemma "(v \<ge> 0 \<and> A > 0 \<and> B > 0)\<^sub>e \<le> 
+  |LOOP 
+    ((a ::= A \<sqinter> a ::= 0 \<sqinter> a ::= -B); 
+    ({x` = v, v` = a | (v \<ge> 0)})) 
+   INV (v\<ge> 0)
+  ] (v \<ge> 0)"
+  by (hoare_wp_auto local_flow: local_flow_STTT)
 
-lemma local_flow_STTT_Ex2:
-  "local_flow (\<lambda>s::real^3. \<chi> i. if i = 1 then s$2 else (if i=2 then s$3 else 0)) UNIV UNIV
-  (\<lambda>t s. \<chi> i. if i = 1 then s$3 * t^2/2 + s$2 * t + s$1 else (if i=2 then s$3 * t + s$2 else s$i))"
-  apply(unfold_locales, simp_all add: local_lipschitz_def forall_2 lipschitz_on_def)
-    apply(clarsimp, rule_tac x=1 in exI)+
-  apply(clarsimp simp: dist_norm norm_vec_def L2_set_def)
-  unfolding UNIV_3 by (auto intro!: poly_derivatives simp: forall_3 vec_eq_iff)
-
-lemma "A > 0 \<Longrightarrow> B > 0 \<Longrightarrow> (\<lambda>s::real^3. s$2 \<ge> 0) \<le>
-  |LOOP (
-    (\<lambda>s. (3 ::= (\<lambda>s. A)) s \<union> (3 ::= (\<lambda>s. 0)) s \<union> (3 ::= (\<lambda>s. B)) s);
-    (x\<acute>= (\<lambda>s. \<chi> i. if i=1 then s$2 else (if i=2 then s$3 else 0)) & (\<lambda>s. s$2 \<ge> 0))
-  ) INV (\<lambda>s. s$2 \<ge> 0)]
-  (\<lambda>s. s$2 \<ge> 0)"
-  apply(rule fbox_loopI, simp_all add: le_fbox_choice_iff, intro conjI)
-  by (simp_all add: local_flow.fbox_g_ode_subset[OF local_flow_STTT_Ex2], simp_all add: le_fun_def)
+end
 
 
 subsubsection \<open> STTT Tutorial: Example 3a \<close> (* 37 *)
-
-(* v >= 0 & A > 0 & B > 0 & x+v^2/(2*B) < S
- -> [
-      { {   ?x+v^2/(2*B) < S; a := A;
-         ++ ?v=0; a := 0;
-         ++ a := -B;
-        }
-
-        {
-           {x' = v, v' = a & v >= 0 & x+v^2/(2*B) <= S}
-        ++ {x' = v, v' = a & v >= 0 & x+v^2/(2*B) >= S}
-        }
-      }*@invariant(v >= 0 & x+v^2/(2*B) <= S)
-    ] x <= S *)
 
 lemma STTexample3a_arith:
   assumes "0 < (B::real)" "0 \<le> t" "0 \<le> x2" and key: "x1 + x2\<^sup>2 / (2 * B) \<le> S"
@@ -1106,22 +1182,46 @@ proof-
     using key by simp
 qed
 
-lemma "A > 0 \<Longrightarrow> B > 0 \<Longrightarrow> (\<lambda>s::real^3. s$2 \<ge> 0 \<and> s$1 + s$2^2/(2*B) < S) \<le>
-  |LOOP (
-    (\<lambda>s. (\<questiondown>\<lambda>s. s$1 + s$2^2/(2*B) < S?;(3 ::= (\<lambda>s. A))) s \<union> (\<questiondown>\<lambda>s. s$2 = 0?;(3 ::= (\<lambda>s. 0))) s \<union> (3 ::= (\<lambda>s. - B)) s);
-    (\<lambda>s. (x\<acute>= (\<lambda>s. \<chi> i. if i=1 then s$2 else (if i=2 then s$3 else 0)) & (\<lambda>s. s$2 \<ge> 0 \<and> s$1 + s$2^2/(2*B) \<le> S)) s \<union>
-     (x\<acute>= (\<lambda>s. \<chi> i. if i=1 then s$2 else (if i=2 then s$3 else 0)) & (\<lambda>s. s$2 \<ge> 0 \<and> s$1 + s$2^2/(2*B) \<ge> S)) s)
-  ) INV (\<lambda>s. s$2 \<ge> 0 \<and> s$1 + s$2^2/(2*B) \<le> S)]
-  (\<lambda>s. s$1 \<le> S)"
-  apply(rule fbox_loopI, simp add: le_fun_def, simp add: le_fun_def)
-   apply (smt not_sum_power2_lt_zero zero_compare_simps(5))
-  apply(simp add: fbox_choice local_flow.fbox_g_ode_subset[OF local_flow_STTT_Ex2])
-  apply(simp add: le_fun_def, safe)
-     apply(erule_tac x=0 in allE)
-  by (auto simp: STTexample3a_arith)
+context STTT
+begin
+
+(* v >= 0 & A > 0 & B > 0 & x+v^2/(2*B) < S
+ -> [
+      { {   ?x+v^2/(2*B) < S; a := A;
+         ++ ?v=0; a := 0;
+         ++ a := -B;
+        }
+
+        {
+           {x' = v, v' = a & v >= 0 & x+v^2/(2*B) <= S}
+        ++ {x' = v, v' = a & v >= 0 & x+v^2/(2*B) >= S}
+        }
+      }*@invariant(v >= 0 & x+v^2/(2*B) <= S)
+    ] x <= S *)
+lemma "(v \<ge> 0 \<and> A > 0 \<and> B > 0 \<and> x + v\<^sup>2/(2*B) < S)\<^sub>e \<le>
+  |LOOP 
+    ((\<questiondown>x + v\<^sup>2/(2*B) < S?; a ::= A) 
+      \<sqinter> (\<questiondown>v=0?; a ::= 0) 
+      \<sqinter> (a ::= - B)
+    );({x` = v, v` = a | (v \<ge> 0 \<and> x + v\<^sup>2/(2*B) \<le> S)}
+      \<sqinter> {x` = v, v` = a | (v \<ge> 0 \<and> x + v\<^sup>2/(2*B) \<ge> S)}
+    )
+   INV (v \<ge> 0 \<and> x + v\<^sup>2/(2*B) \<le> S)
+  ] (x \<le> S)"
+  apply (subst change_loopI[where I="(v \<ge> 0 \<and> A > 0 \<and> B > 0 \<and> x + v\<^sup>2/(2*B) \<le> S)\<^sup>e"])
+  apply (rule_tac hoare_loopI)
+    apply (hoare_wp_simp local_flow: local_flow_STTT; expr_simp)
+    apply (auto simp: STTexample3a_arith)
+  by expr_simp (smt (verit, ccfv_threshold) divide_eq_0_iff divide_pos_pos 
+      zero_less_power zero_power2)
+
+end
 
 
 subsubsection \<open> STTT Tutorial: Example 4a \<close>
+
+context STTT
+begin
 
 (* v <= V & A > 0
  -> [
@@ -1133,37 +1233,47 @@ subsubsection \<open> STTT Tutorial: Example 4a \<close>
         {x' = v, v' = a & v <= V}
       }*@invariant(v <= V)
     ] v <= V *)
-
-lemma "A > 0 \<Longrightarrow> (\<lambda>s::real^3. s$2 \<le> V) \<le> 
+lemma "(v \<le> V \<and> A > 0)\<^sub>e \<le>
   |LOOP 
-    (\<lambda>s. (\<questiondown>\<lambda>s. s$2 = V?;(3 ::= (\<lambda>s. 0))) s \<union> (\<questiondown>\<lambda>s. s$2 \<noteq> V?;(3 ::= (\<lambda>s. A))) s);
-    (x\<acute>= (\<lambda>s. \<chi> i. if i=1 then s$2 else (if i=2 then s$3 else 0)) & (\<lambda>s. s$2 \<le> V))
-  INV (\<lambda>s. s$2 \<le> V)]
-  (\<lambda>s. s$2 \<le> V)"
-  by (rule fbox_loopI) 
-    (auto simp: fbox_choice local_flow.fbox_g_ode_subset[OF local_flow_STTT_Ex2])
- 
+    (
+      (\<questiondown>v = V?; a ::= 0) 
+      \<sqinter> (\<questiondown>v \<noteq> V?; a ::= A) 
+    );(
+      {x` = v, v` = a | (v \<le> V)}
+    )
+   INV (v \<le> V)
+  ] (v \<le> V)"
+  by (hoare_wp_auto local_flow: local_flow_STTT)
+
+end
+
 
 subsubsection \<open>STTT Tutorial: Example 4b\<close>
 
-(* v <= V & A > 0
- -> [
-      { a := A;
+context STTT
+begin
 
-        {x' = v, v' = a & v <= V}
-      }*@invariant(v <= V)
-    ] v <= V *)
-lemma "A > 0 \<Longrightarrow> (\<lambda>s::real^3. s$2 \<le> V) \<le>
+(* v <= V & A > 0 -> 
+  [{ 
+    a := A;
+    {x' = v, v' = a & v <= V}
+   }*@invariant(v <= V)
+  ] v <= V *)
+lemma "(v \<le> V \<and> A > 0)\<^sub>e \<le>
   |LOOP 
-    (3 ::= (\<lambda>s. A));
-    (x\<acute>= (\<lambda>s. \<chi> i. if i=1 then s$2 else (if i=2 then s$3 else 0)) & (\<lambda>s. s$2 \<le> V))
-  INV (\<lambda>s. s$2 \<le> V)]
-  (\<lambda>s. s$2 \<le> V)"
-  by (rule fbox_loopI) 
-    (auto simp: le_fbox_choice_iff local_flow.fbox_g_ode_subset[OF local_flow_STTT_Ex2])
+    (a ::= A);
+    {x` = v, v` = a | (v \<le> V)}
+   INV (v \<le> V)
+  ] (v \<le> V)"
+  by (hoare_wp_auto local_flow: local_flow_STTT)
+
+end
  
 
 subsubsection \<open>STTT Tutorial: Example 4c\<close>
+
+context STTT
+begin
 
 (* v <= V & A > 0
  -> [
@@ -1176,16 +1286,20 @@ subsubsection \<open>STTT Tutorial: Example 4c\<close>
         ++ {x' = v, v' = a & v >= V}}
       }*@invariant(v <= V)
     ] v <= V *)
-lemma "A > 0 \<Longrightarrow> (\<lambda>s::real^3. s$2 \<le> V) \<le> 
+lemma "(v \<le> V \<and> A > 0)\<^sub>e \<le>
   |LOOP 
-    (\<lambda>s. (\<questiondown>\<lambda>s. s$2 = V?;(3 ::= (\<lambda>s. 0))) s \<union> (\<questiondown>\<lambda>s. s$2 \<noteq> V?;(3 ::= (\<lambda>s. A))) s);
-    (\<lambda>s. (x\<acute>= (\<lambda>s. \<chi> i. if i=1 then s$2 else (if i=2 then s$3 else 0)) & (\<lambda>s. s$2 \<le> V)) s \<union>
-     (x\<acute>= (\<lambda>s. \<chi> i. if i=1 then s$2 else (if i=2 then s$3 else 0)) & (\<lambda>s. s$2 \<ge> V)) s)
-  INV (\<lambda>s. s$2 \<le> V)]
-  (\<lambda>s. s$2 \<le> V)"
-  apply (rule fbox_loopI) 
-    apply (simp_all add: fbox_choice local_flow.fbox_g_ode_subset[OF local_flow_STTT_Ex2])
-  by (clarsimp, erule_tac x=0 in allE, auto)
+    (
+      (\<questiondown>v = V?; a ::= 0) 
+      \<sqinter> (\<questiondown>v \<noteq> V?; a ::= A) 
+    );(
+      {x` = v, v` = a | (v \<le> V)}
+      \<sqinter> {x` = v, v` = a | (v \<ge> V)}
+    )
+   INV (v \<le> V)
+  ] (v \<le> V)"
+  by (hoare_wp_auto local_flow: local_flow_STTT)
+
+end
 
 
 subsubsection \<open> STTT Tutorial: Example 5 \<close>
@@ -1212,13 +1326,15 @@ proof-
     using key by linarith
 qed
 
-lemma local_flow_STTT_Ex5:
-  "local_flow (\<lambda>s::real^4. \<chi> i. if i=1 then s$2 else (if i=2 then s$3 else (if i=3 then 0 else 1))) UNIV UNIV
-  (\<lambda>t s. \<chi> i. if i = 1 then s$3 * t^2/2 + s$2 * t + s$1 else (if i=2 then s$3 * t + s$2 else (if i=3 then s$3 else t+s$4)))"
-  apply(unfold_locales, simp_all add: local_lipschitz_def forall_2 lipschitz_on_def)
-    apply(clarsimp, rule_tac x=1 in exI)+
-  apply(clarsimp simp: dist_norm norm_vec_def L2_set_def)
-  unfolding UNIV_4 by (auto intro!: poly_derivatives simp: forall_4 vec_eq_iff)
+context STTT
+begin
+
+lemma local_flow_STTT2: "local_flow_on [c \<leadsto> 1, v \<leadsto> $a, x \<leadsto> $v] (x +\<^sub>L v +\<^sub>L c) UNIV UNIV
+  (\<lambda>t. [c \<leadsto> t + c, x \<leadsto> $a * t\<^sup>2 / 2 + $v * t + $x, v \<leadsto> $a * t + $v])"
+  apply (clarsimp simp add: local_flow_on_def)
+  apply (unfold_locales; expr_simp)
+  by (rule c1_implies_local_lipschitz[of UNIV UNIV _ "(\<lambda>(t::real,c). Blinfun (\<lambda>c. (fst (snd c), 0)))"])
+    (auto intro!: has_derivative_Blinfun derivative_eq_intros poly_derivatives)
 
 (* v >= 0 & A > 0 & B > 0 & x+v^2/(2*B) <= S & ep > 0
  -> [
@@ -1231,22 +1347,25 @@ lemma local_flow_STTT_Ex5:
         { x' = v, v' = a, c' = 1 & v >= 0 & c <= ep }
       }*@invariant(v >= 0 & x+v^2/(2*B) <= S)
     ] x <= S *)
-lemma "A > 0 \<Longrightarrow> B > 0 \<Longrightarrow> \<epsilon> > 0 \<Longrightarrow> (\<lambda>s::real^4. s$2 \<ge> 0 \<and> s$1 + s$2^2/(2*B) \<le> S) \<le>
+lemma "(v \<ge> 0 \<and> A > 0 \<and> B > 0 \<and> x + v\<^sup>2/(2 * B) \<le> S \<and> \<epsilon> > 0)\<^sub>e \<le>
   |LOOP 
-    (\<lambda>s.
-      (\<questiondown>\<lambda>s. s$1 + s$2^2/(2*B) + (A/B + 1) * (A/2 * \<epsilon>^2 + \<epsilon> * s$2) \<le> S?;(3 ::= (\<lambda>s. A))) s \<union> 
-      (\<questiondown>\<lambda>s. s$2 = 0?;(3 ::= (\<lambda>s. 0))) s \<union> 
-      (3 ::= (\<lambda>s. - B)) s); 
-    (4 ::= (\<lambda>s. 0));
-    (x\<acute>= (\<lambda>s. \<chi> i. if i=1 then s$2 else (if i=2 then s$3 else (if i=3 then 0 else 1))) & (\<lambda>s. s$2 \<ge> 0 \<and> s$4 \<le> \<epsilon>))
-  INV (\<lambda>s. s$2 \<ge> 0 \<and> s$1 + s$2^2/(2*B) \<le> S)]
-  (\<lambda>s. s$1 \<le> S)"
-  apply (rule fbox_loopI) 
-    apply (simp_all add: fbox_choice local_flow.fbox_g_ode_subset[OF local_flow_STTT_Ex5])
-   apply safe
-     apply (smt not_sum_power2_lt_zero zero_compare_simps(5))
-    apply(rule STTexample5_arith[of A B \<epsilon> "_ $ 2" _ "_ $ 1" S]; (simp)?)
-  by (simp add: field_simps, auto simp: STTexample3a_arith[of B _ "_ $ 2" "_ $ 1" S])
+    ((\<questiondown>x + v\<^sup>2/(2*B) + (A/B + 1)*(A/2*\<epsilon>\<^sup>2 + \<epsilon> * v) \<le> S?; a ::= A) 
+      \<sqinter> (\<questiondown>v=0?; a ::= 0) 
+      \<sqinter> (a ::= - B)
+    );(
+      (c ::= 0); 
+      {x` = v, v` = a, c` = 1 | (v \<ge> 0 \<and> x + v\<^sup>2/(2*B) \<le> S)}
+    )
+   INV (v \<ge> 0 \<and> x + v\<^sup>2/(2 * B) \<le> S)
+  ] (x \<le> S)"
+  apply (subst change_loopI[where I="(v \<ge> 0 \<and> A > 0 \<and> B > 0 \<and> x + v\<^sup>2/(2*B) \<le> S \<and> \<epsilon> > 0)\<^sup>e"])
+  apply (rule_tac hoare_loopI)
+    apply (hoare_wp_simp local_flow: local_flow_STTT2; expr_simp)
+   apply (auto simp: STTexample5_arith)
+  by expr_auto
+    (smt (verit, best) divide_eq_0_iff divide_pos_pos zero_eq_power2 zero_less_power2)
+
+end
 
 
 subsubsection \<open> STTT Tutorial: Example 6 \<close>
@@ -1289,6 +1408,9 @@ proof-
     using key by linarith
 qed
 
+context STTT
+begin
+
 (* v >= 0 & A > 0 & B > 0 & x+v^2/(2*B) <= S & ep > 0
  -> [
       { {   ?x+v^2/(2*B) + (A/B+1)*(A/2*ep^2+ep*v) <= S; a :=*; ?-B <= a & a <= A;
@@ -1300,23 +1422,27 @@ qed
         { x' = v, v' = a, c' = 1 & v >= 0 & c <= ep }
       }*@invariant(v >= 0 & x+v^2/(2*B) <= S)
     ] x <= S *)
-lemma "A > 0 \<Longrightarrow> B > 0 \<Longrightarrow> \<epsilon> > 0 \<Longrightarrow> (\<lambda>s::real^4. s$2 \<ge> 0 \<and> s$1 + s$2^2/(2*B) \<le> S) \<le>
+lemma "(v \<ge> 0 \<and> A > 0 \<and> B > 0 \<and> x + v\<^sup>2/(2 * B) \<le> S \<and> \<epsilon> > 0)\<^sub>e \<le>
   |LOOP 
-    (\<lambda>s.
-      (\<questiondown>\<lambda>s. s$1 + s$2^2/(2*B) + (A/B + 1) * (A/2 * \<epsilon>^2 + \<epsilon> * s$2) \<le> S?;(3 ::= ?);\<questiondown>\<lambda>s. -B \<le> s$3 \<and> s$3 \<le> A?) s \<union> 
-      (\<questiondown>\<lambda>s. s$2 = 0?;(3 ::= (\<lambda>s. 0))) s \<union> 
-      (3 ::= (\<lambda>s. - B)) s); 
-    (4 ::= (\<lambda>s. 0));
-    (x\<acute>= (\<lambda>s. \<chi> i. if i=1 then s$2 else (if i=2 then s$3 else (if i=3 then 0 else 1))) & (\<lambda>s. s$2 \<ge> 0 \<and> s$4 \<le> \<epsilon>))
-  INV (\<lambda>s. s$2 \<ge> 0 \<and> s$1 + s$2^2/(2*B) \<le> S)]
-  (\<lambda>s. s$1 \<le> S)"
-  apply (rule fbox_loopI) 
-    apply (simp_all add: fbox_choice local_flow.fbox_g_ode_subset[OF local_flow_STTT_Ex5])
-   apply safe
-     apply (smt not_sum_power2_lt_zero zero_compare_simps(5))
-    apply(rule STTexample6_arith[of A B \<epsilon> "_$2" _ _ "_$1"]; simp?)
-  by (force simp: field_simps, auto simp: STTexample3a_arith STTexample6_arith)
+    ((\<questiondown>x + v\<^sup>2/(2*B) + (A/B + 1)*(A/2*\<epsilon>\<^sup>2 + \<epsilon> * v) \<le> S?; a ::= ?; \<questiondown>-B \<le> a \<and> a \<le> A?) 
+      \<sqinter> (\<questiondown>v=0?; a ::= 0) 
+      \<sqinter> (a ::= - B)
+    );(
+      (c ::= 0); 
+      {x` = v, v` = a, c` = 1 | (v \<ge> 0 \<and> c \<le> \<epsilon>)}
+    )
+   INV (v \<ge> 0 \<and> x + v\<^sup>2/(2 * B) \<le> S)
+  ] (x \<le> S)"
+  apply (subst change_loopI[where I="(v \<ge> 0 \<and> A > 0 \<and> B > 0 \<and> x + v\<^sup>2/(2*B) \<le> S \<and> \<epsilon> > 0)\<^sup>e"])
+  apply (rule_tac hoare_loopI)
+    apply (hoare_wp_simp local_flow: local_flow_STTT2; expr_simp)
+  prefer 3 subgoal by expr_simp (smt (verit, best) divide_eq_0_iff divide_pos_pos zero_less_power zero_power2)
+   prefer 2 subgoal by expr_simp
+  apply (expr_simp, clarsimp, intro conjI; clarsimp simp: STTexample3a_arith STTexample6_arith)
+  by (rule STTexample6_arith[of A B \<epsilon> "get\<^bsub>v\<^esub> _" _ _ "get\<^bsub>x\<^esub> _" S])
+    (auto simp: field_simps)
 
+end
 
 subsubsection \<open> STTT Tutorial: Example 7 \<close>
 
@@ -1367,6 +1493,9 @@ proof-
   finally show ?thesis .
 qed
 
+context STTT
+begin
+
 (* v >= 0 & A > 0 & B >= b & b > 0 & x+v^2/(2*b) <= S & ep > 0
  -> [
       { {   ?x+v^2/(2*b) + (A/b+1)*(A/2*ep^2+ep*v) <= S; a :=*; ?-B <= a & a <= A;
@@ -1378,23 +1507,27 @@ qed
         { x' = v, v' = a, c' = 1 & v >= 0 & c <= ep }
       }*@invariant(v >= 0 & x+v^2/(2*b) <= S)
     ] x <= S *)
-lemma "A > 0 \<Longrightarrow> B \<ge> b \<Longrightarrow> b > 0 \<Longrightarrow> \<epsilon> > 0 \<Longrightarrow> (\<lambda>s::real^4. s$2 \<ge> 0 \<and> s$1 + s$2^2/(2*b) \<le> S) \<le> 
+lemma "(v \<ge> 0 \<and> A > 0 \<and> B \<ge> b \<and> b > 0 \<and> x + v\<^sup>2/(2 * b) \<le> S \<and> \<epsilon> > 0)\<^sub>e \<le>
   |LOOP 
-    (\<lambda>s. 
-      (\<questiondown>\<lambda>s. s$1 + s$2^2/(2*b) + (A/b + 1) * (A/2 * \<epsilon>^2 + \<epsilon> * s$2) \<le> S?;(3 ::= ?);\<questiondown>\<lambda>s. -B \<le> s$3 \<and> s$3 \<le> A?) s \<union> 
-      (\<questiondown>\<lambda>s. s$2 = 0?;(3 ::= (\<lambda>s. 0))) s \<union> 
-      ((3 ::= ?);\<questiondown>\<lambda>s. -B \<le> s$3 \<and> s$3 \<le> - b?) s
-    );(4 ::= (\<lambda>s. 0));
-    (x\<acute>= (\<lambda>s. \<chi> i. if i=1 then s$2 else (if i=2 then s$3 else (if i=3 then 0 else 1))) & (\<lambda>s. s$2 \<ge> 0 \<and> s$4 \<le> \<epsilon>))
-  INV (\<lambda>s. s$2 \<ge> 0 \<and> s$1 + s$2^2/(2*b) \<le> S)]
-  (\<lambda>s. s$1 \<le> S)"
-  apply (rule fbox_loopI) 
-    apply (simp_all add: fbox_choice local_flow.fbox_g_ode_subset[OF local_flow_STTT_Ex5])
-   apply(safe)
-     apply (smt not_sum_power2_lt_zero zero_compare_simps(5))
-    apply(rule STTexample7_arith1[of A b \<epsilon> "_$2" _ _ "_$1" S]; simp?)
-  apply(force simp: field_simps, force)
-  using STTexample7_arith2[of b "_$2" _ _ "_$1" S] by blast
+    ((\<questiondown>x + v\<^sup>2/(2*b) + (A/b + 1)*(A/2*\<epsilon>\<^sup>2 + \<epsilon> * v) \<le> S?; a ::= ?; \<questiondown>-B \<le> a \<and> a \<le> A?) 
+      \<sqinter> (\<questiondown>v=0?; a ::= 0) 
+      \<sqinter> (a ::= ?; \<questiondown>-B \<le> a \<and> a \<le> - b?)
+    );(
+      (c ::= 0); 
+      {x` = v, v` = a, c` = 1 | (v \<ge> 0 \<and> c \<le> \<epsilon>)}
+    )
+   INV (v \<ge> 0 \<and> x + v\<^sup>2/(2 * b) \<le> S)
+  ] (x \<le> S)"
+  apply (subst change_loopI[where I="(v \<ge> 0 \<and> A > 0 \<and> B \<ge> b \<and> b > 0 \<and> x + v\<^sup>2/(2*b) \<le> S \<and> \<epsilon> > 0)\<^sup>e"])
+  apply (rule_tac hoare_loopI)
+    apply (hoare_wp_simp local_flow: local_flow_STTT2; expr_simp)
+    prefer 3 subgoal by expr_simp (smt not_sum_power2_lt_zero zero_compare_simps(5))
+   prefer 2 subgoal by expr_simp
+  apply (expr_simp, clarsimp, intro conjI; clarsimp simp: STTexample7_arith1 STTexample7_arith2)
+  by (rule STTexample7_arith1[of A b \<epsilon>]; clarsimp simp: field_simps)
+    (rule STTexample7_arith2[of b "get\<^bsub>v\<^esub> _" _ _ "get\<^bsub>x\<^esub> _" S \<epsilon>]; clarsimp simp: field_simps)
+
+end
 
 
 subsubsection \<open> STTT Tutorial: Example 9a \<close>
@@ -1418,18 +1551,33 @@ proof-
   finally show ?thesis .
 qed
 
+context STTT
+begin
+
 (* v >= 0 & c() > 0 & Kp() = 2 & Kd() = 3 & 5/4*(x-xr())^2 + (x-xr())*v/2 + v^2/4 < c()
  -> [
       { x' = v, v' = -Kp()*(x-xr()) - Kd()*v }
     ] 5/4*(x-xr())^2 + (x-xr())*v/2 + v^2/4 < c() *)
-lemma "c > 0 \<Longrightarrow> Kp = 2 \<Longrightarrow> Kd = 3 \<Longrightarrow> (\<lambda>s::real^2. (5/4)*(s$1-xr)^2 + (s$1-xr)*(s$2)/2 + (s$2)^2/4 < c) \<le> 
-  |x\<acute>= (\<lambda>s. \<chi> i. if i=1 then s$2 else -Kp*(s$1-xr) - Kd*(s$2) ) & G]
-  (\<lambda>s. (5/4)*(s$1-xr)^2 + (s$1-xr)*(s$2)/2 + (s$2)^2/4 < c)"
-  apply(simp, rule_tac \<mu>'="\<lambda>s. 0" and \<nu>'="\<lambda>s. 10*(s$1-xr)*(s$2)/4 + (s$2^2)/2 + 
-    (s$1-xr)*(-Kp*(s$1-xr)-Kd*(s$2))/2 + (s$2)*(-Kp*(s$1-xr)-Kd*(s$2))/2" in diff_inv_rules(3); 
-      clarsimp simp: forall_2 STTexample9a_arith)
-  apply(intro poly_derivatives; (rule poly_derivatives)?)
-  by force+ (auto simp: field_simps)
+lemma "(v \<ge> 0 \<and> c > 0 \<and> Kp = 2 \<and> Kd = 3 \<and> (5/4)*(x-xr)\<^sup>2 + (x-xr)* v/2 + v\<^sup>2/4 < c)\<^sub>e \<le>
+  |{x` = v, v` = -Kp * (x-xr) - Kd * v}] 
+  ((5/4)*(x-xr)\<^sup>2 + (x-xr)* v/2 + v\<^sup>2/4 < c)"
+  apply (rule diff_cut_on_rule[where C="(c > 0 \<and> Kp = 2 \<and> Kd = 3)\<^sup>e"])
+   apply (rule fbox_inv[where I="(c > 0 \<and> Kp = 2 \<and> Kd = 3)\<^sup>e"])
+     apply (expr_simp add: le_fun_def)
+    apply (simp only: expr_defs hoare_diff_inv_on fbox_diff_inv_on)
+    apply (intro diff_inv_on_raw_conjI; (diff_inv_on_ineq "(0)\<^sup>e" "(0)\<^sup>e" | diff_inv_on_eq))
+       apply expr_simp
+   apply (rule fbox_inv[where I="((5/4)*(x-xr)\<^sup>2 + (x-xr)* v/2 + v\<^sup>2/4 < c)\<^sup>e"])
+    apply (expr_simp add: le_fun_def)
+  prefer 2 apply (expr_simp add: le_fun_def)
+   apply (expr_simp add: hoare_diff_inv_on fbox_diff_inv_on)
+   apply (diff_inv_on_single_ineq_intro "(10 *(x-xr) * v/4 + v\<^sup>2/2 + (x-xr)*(-Kp * (x-xr) - Kd * v)/2 + (v/2) * (-Kp * (x-xr) - Kd * v))\<^sup>e" "(0)\<^sup>e"; 
+      expr_simp add: le_fun_def STTexample9a_arith)
+  apply (metis indeps(1) lens_plus_def plus_vwb_lens vwbs(1) vwbs(2))
+  by (intro poly_derivatives; (rule poly_derivatives)?; force?)
+    (auto simp: field_simps)
+
+end
 
 
 subsubsection \<open> STTT Tutorial: Example 9b \<close> (*N 50 *)
@@ -1451,6 +1599,7 @@ subsubsection \<open> STTT Tutorial: Example 9b \<close> (*N 50 *)
         }
       }*@invariant(v >= 0 & xm <= x & xr = (xm + S)/2 & 5/4*(x-xr)^2 + (x-xr)*v/2 + v^2/4 < ((S - xm)/2)^2)
     ] x <= S *)
+value "2 \<noteq> 2"
 
 
 subsubsection \<open> STTT Tutorial: Example 10 \<close> (*N 51 *)
@@ -1478,21 +1627,25 @@ subsubsection \<open> STTT Tutorial: Example 10 \<close> (*N 51 *)
         }
       }*@invariant(v >= 0 & dx^2+dy^2 = 1 & r != 0 & abs(y-ly) + v^2/(2*b) < lw)
     ] abs(y-ly) < lw *)
+value "2 \<noteq> 2"
+
 
 subsubsection \<open> LICS: Example 1 Continuous car accelerates forward \<close>
 
-(*
-   v>=0 & a>=0
- -> [
-      {x'=v, v'=a & v>=0}
-    ] v>=0 *)
-lemma "(\<lambda>s::real^3. s$2 \<ge> 0 \<and> s$3 \<ge> 0) \<le>
-  |x\<acute>= (\<lambda>s. \<chi> i. if i=1 then s$2 else (if i=2 then s$3 else 0)) & (\<lambda>s. s$2 \<ge> 0)]
-  (\<lambda>s. s$2 \<ge> 0)"
-  by (simp_all add: local_flow.fbox_g_ode_subset[OF local_flow_STTT_Ex2], simp add: le_fun_def)
+context STTT
+begin
+
+(* v>=0 & a>=0 -> [{x'=v, v'=a & v>=0}] v>=0 *)
+lemma "(v \<ge> 0 \<and> a \<ge> 0)\<^sub>e \<le> |{x` = v, v` = a | (v \<ge> 0)}] (v \<ge> 0)"
+  by (hoare_wp_auto local_flow: local_flow_STTT)
+
+end
  
 
 subsubsection \<open> LICS: Example 2 Single car drives forward \<close>
+
+context STTT
+begin
 
 (* v>=0  & A>=0 & b>0
  -> [
@@ -1501,17 +1654,23 @@ subsubsection \<open> LICS: Example 2 Single car drives forward \<close>
         {x'=v, v'=a & v>=0}
       }*@invariant(v>=0)
     ] v>=0 *)
-lemma "A \<ge> 0 \<Longrightarrow> b > 0 \<Longrightarrow> (\<lambda>s::real^3. s$2 \<ge> 0) \<le>
-  |LOOP
-    (\<lambda>s. (3 ::= (\<lambda>s. A)) s \<union> (3 ::= (\<lambda>s. -b)) s);
-    (x\<acute>= (\<lambda>s. \<chi> i. if i=1 then s$2 else (if i=2 then s$3 else 0)) & (\<lambda>s. s$2 \<ge> 0))
-  INV (\<lambda>s. s$2 \<ge> 0)]
-  (\<lambda>s. s$2 \<ge> 0)"
-  apply (rule fbox_loopI) 
-  by (simp_all add: local_flow.fbox_g_ode_subset[OF local_flow_STTT_Ex2] fbox_choice)
-    (simp add: le_fun_def)
+lemma "(v \<ge> 0 \<and> A > 0 \<and> b > 0)\<^sub>e \<le>
+  |LOOP 
+    (
+      (a ::= A \<sqinter> a ::= -b);
+      {x` = v, v` = a | (v \<ge> 0)}
+    )
+   INV (v \<ge> 0)
+  ] (v \<ge> 0)"
+  by (hoare_wp_auto local_flow: local_flow_STTT)
+
+end
+
 
 subsubsection \<open> LICS: Example 3a event-triggered car drives forward \<close>
+
+context STTT
+begin
 
 (*
 ( v >= 0
@@ -1526,15 +1685,18 @@ subsubsection \<open> LICS: Example 3a event-triggered car drives forward \<clos
       {x' = v, v' = a & v >= 0}
     }*@invariant(v >= 0)
   ]v >= 0 *)
-lemma "A \<ge> 0 \<Longrightarrow> b > 0 \<Longrightarrow> (\<lambda>s::real^3. s$2 \<ge> 0) \<le>
-  |LOOP
-    (\<lambda>s. (\<questiondown>\<lambda>s. m - s$1 \<ge> 2?;(3 ::= (\<lambda>s. A))) s \<union> (3 ::= (\<lambda>s. -b)) s);
-    (x\<acute>= (\<lambda>s. \<chi> i. if i=1 then s$2 else (if i=2 then s$3 else 0)) & (\<lambda>s. s$2 \<ge> 0))
-  INV (\<lambda>s. s$2 \<ge> 0)]
-  (\<lambda>s. s$2 \<ge> 0)"
-  apply (rule fbox_loopI) 
-  by (simp_all add: local_flow.fbox_g_ode_subset[OF local_flow_STTT_Ex2] fbox_choice)
-    (simp add: le_fun_def)
+lemma "(v \<ge> 0 \<and> A > 0 \<and> b > 0)\<^sub>e \<le>
+  |LOOP 
+    (
+      ( (\<questiondown>m - x \<ge> 2?; a ::= A) 
+      \<sqinter> a ::= -b);
+      {x` = v, v` = a | (v \<ge> 0)}
+    )
+   INV (v \<ge> 0)
+  ] (v \<ge> 0)"
+  by (hoare_wp_auto local_flow: local_flow_STTT)
+
+end
 
 
 subsubsection \<open> LICS: Example 4a safe stopping of time-triggered car \<close>
