HS_Preliminaries.thy
@@ -35,7 +35,39 @@ no_notation has_derivative ("(1(D _ \<mapsto> (_))/ _)" [65,65] 61)
 
 end
 
-unbundle derivative_notation \<comment> \<open> enable notation \<close>
+text \<open>Special syntax for cubes, power to the 4th and 5th. \<close>
+abbreviation power3 :: "'a::power \<Rightarrow> 'a"  ("(_\<^sup>3)" [1000] 999)
+  where "x\<^sup>3 \<equiv> x ^ 3"
+
+abbreviation power4 :: "'a::power \<Rightarrow> 'a"  ("(_\<^sup>4)" [1000] 999)
+  where "x\<^sup>4 \<equiv> x ^ 4"
+
+abbreviation power5 :: "'a::power \<Rightarrow> 'a"  ("(_\<^sup>5)" [1000] 999)
+  where "x\<^sup>5 \<equiv> x ^ 5"
+
+bundle power_notation
+begin
+
+notation power2 ("(_\<^sup>2)" [1000] 999)
+  and power3 ("(_\<^sup>3)" [1000] 999) 
+  and power4 ("(_\<^sup>4)" [1000] 999)
+  and power5 ("(_\<^sup>5)" [1000] 999)
+
+end
+
+bundle power_no_notation
+begin
+
+no_notation power2 ("(_\<^sup>2)" [1000] 999)
+  and power3 ("(_\<^sup>3)" [1000] 999) 
+  and power4 ("(_\<^sup>4)" [1000] 999)
+  and power5 ("(_\<^sup>5)" [1000] 999)
+
+end
+
+unbundle power_no_notation
+unbundle derivative_notation
+unbundle power_notation \<comment> \<open> enable notation \<close>
 
 
 subsection \<open> Real vector arithmetic \<close>
